\documentclass[11pt, oneside]{article}   	% use "amsart" instead of "article" for AMSLaTeX format
\usepackage{geometry}                		% See geometry.pdf to learn the layout options. There are lots.
\geometry{letterpaper}                   		% ... or a4paper or a5paper or ... 
%\geometry{landscape}                		% Activate for rotated page geometry
%\usepackage[parfill]{parskip}    		% Activate to begin paragraphs with an empty line rather than an indent
\usepackage{graphicx}				% Use pdf, png, jpg, or epsÂ§ with pdflatex; use eps in DVI mode
								% TeX will automatically convert eps --> pdf in pdflatex		
\usepackage{amssymb}

%SetFonts

%SetFonts


\title{Problem Three}
\author{Michael Cai}
%\date{}							% Activate to display a given date or no date

\begin{document}
\maketitle
\section{}
%\subsection{}
Output

$y_t = e^{z_t}k_t^\alpha$

Suppose $y_t$ and $k_t$ changes around their steady states $y$ and $k$

$\hat{y_t} = log(\frac{y_t}{y})$ 

$y_t = ye^{\hat{y_t}}$ and $k_t$ follows the same form.

Then $ye^{\hat{y_t}} = e^{z_t}(ke^{{\hat{k_t}})^{\alpha}}$

In the steady-state $z_t = 0$, thus $e^{z_t} = 1$

$\therefore y = k^\alpha$

Thus dividing both sides by $y/k^\alpha$ equivalently, we get:

$= e^{\hat{y_t}} = e^{z_t}(e^{\hat{k_t}})^\alpha$

And taking logs we get:

$\hat{y_t} = z_t + \alpha \hat{k_t}$

Capital

$k_{t+1} = (1-\delta)k_t + se^{z_t} k_t^\alpha$

$k_t$ and $k_{t+1}$ changes around its steady state k.

Therefore:

$ke^{\widehat{k_{t+1}}} = (1-\delta)ke^{\hat{k_t}} + se^{z_t} (ke^{\hat{k_t}})^\alpha$

Dividing by $k$ we get:

$e^{\widehat{k_{t+1}}} = (1-\delta)e^{\hat{k_t}} + \frac{sk^\alpha}{k}e^{z_t}(e^{\hat{k_t}})^\alpha$

Recall: $k_{t+1} = (1-\delta)k_t + sy_t$

In the steady-state: 

$k = (1-\delta)k + sy$

$k - (1-\delta)k = sy$

$\delta k = sy$

Because $y = k^\alpha$

$\delta k = sk^\alpha$

$\delta = \frac{sk^\alpha}{k}$

Thus replacing $\frac{sk^\alpha}{k}$ in our last equation with $\delta$ we get:

$e^{\widehat{k_{t+1}}} = (1-\delta)e^{\hat{k_t}} + \delta e^{z_t}(e^{\hat{k_t}})^\alpha$

Recall from the Taylor Series expansion of $e^x$

$e^x = 1 + x + \frac{1}{2}x^2 + ...$

$ \approx 1+x$

Thus $e^{\widehat{k_{t+1}}} \approx 1+\widehat{k_{t+1}} = (1-\delta)(1+\hat{k_t}) + \delta (1+z_t+\alpha \hat{k_t})$

$=(1-\delta) + (1-\delta)\hat{k_t} + \delta + delta(z_t + \alpha \hat{k_t})$

$\widehat{k_{t+1}} = (1-\delta)\hat{k_t} + \delta z_t + \alpha \delta \hat{k_t}$

$\widehat{k_{t+1}} = \delta z_t + (1-\delta+\alpha \delta)\hat{k_t}$

\section{}

Expressing as ARMA processes

$\widehat{k_{t+1}} = (1-\delta-\alpha \delta)\hat{k_t} + \delta z_t$

Recall:

$z_t = \rho z_{t-1} + w_t$

$=\rho L z_t + w_t$

$(1-\rho L)z_t = w_t$

$z_t = \frac{1}{1-\rho L}w_t$

Plugging this back into our equation for $\widehat{k_{t+1}}$

$\widehat{k_{t+1}} = (1-\delta-\alpha \delta)\hat{k_t} + \delta(\frac{1}{1-\rho L}w_t)$

Then plugging in the lag operator, $L$

$\widehat{k_{t+1}} = (1-\delta-\alpha \delta)L \widehat{k_{t+1}} + \delta(\frac{1}{1-\rho L}w_t)$

$\widehat{k_{t+1}} -  (1-\delta-\alpha \delta)L \widehat{k_{t+1}} = \delta(\frac{1}{1-\rho L}w_t)$

$[1-(1-\delta-\alpha \delta)L] \widehat{k_{t+1}} = \delta(\frac{1}{1-\rho L}w_t)$

$\widehat{k_{t+1}} = \delta(\frac{1}{[1-(1-\delta-\alpha \delta)L] (1-\rho L)})w_t$

Lets denote $1-(1-\delta-\alpha \delta)L$ as $\rho_1$ and the previous $\rho$ as $\rho_2$, which will make the equation of the form:

$\widehat{k_{t+1}} = \delta(\frac{1}{[1-\rho_1 L] (1-\rho_2 L)})w_t$

$=(1-\rho_1 L)(1-\rho_2 L)\widehat{k_{t+1}} = \delta w_t$

$[1-(\rho_1 + \rho_2)L + \rho_1 \rho_2 L^2]\widehat{k_{t+1}} = \delta w_t$

$\widehat{k_{t+1}} - (\rho_1 + \rho_2)\hat{k_t} + \rho_1 \rho_2 \widehat{k_{t-1}} = \delta w_t$

Let us denote $\rho_1 + \rho_2$ as $\phi_1$ and $\rho_1 \rho_2$ as $\phi_2$

Now $\widehat{k_{t+1}}$ is rewritten as an AR(2) process:

$\widehat{k_{t+1}} = \phi_1 \hat{k_t} + \phi_2 \hat{k_{t-1}} + \delta w_t$

\end{document}  